@prefix : <http://www.geoscienceontology.org/svu#> .
@prefix owl: <http://www.w3.org/2002/07/owl#> .
@prefix rdf: <http://www.w3.org/1999/02/22-rdf-syntax-ns#> .
@prefix xml: <http://www.w3.org/XML/1998/namespace> .
@prefix xsd: <http://www.w3.org/2001/XMLSchema#> .
@prefix rdfs: <http://www.w3.org/2000/01/rdf-schema#> .

<http://www.geoscienceontology.org/svu> a owl:Ontology ;
	rdfs:comment "Scientific Variables Ontology: Upper Ontology. This Ontology defines the core classes and design patterns for building variables. Class individuals are declared in the lower ontology." .
# 
# 
# #################################################################
# #
# #    Annotation properties
# #
# #################################################################
# 
# 
# http://www.geoscienceontology.org/svu#hasAssociatedWikipediaPage

:hasAssociatedWikipediaPage a owl:AnnotationProperty ;
	rdfs:comment "Points to a URL identifying a related Wikipedia Page. Wikipedia pages are used to retrieve narrative, documentation information about entitites in the ontology when available. Wikipedia URLs are not equivalent IRIs." ;
	rdfs:subPropertyOf rdfs:comment .
# 
# http://www.geoscienceontology.org/svu#hasNominalization

:hasNominalization a owl:AnnotationProperty ;
	rdfs:subPropertyOf rdfs:label .
# 
# http://www.geoscienceontology.org/svu#hasPresentParticiple

:hasPresentParticiple a owl:AnnotationProperty ;
	rdfs:subPropertyOf rdfs:label .
# 
# 
# 
# #################################################################
# #
# #    Object Properties
# #
# #################################################################
# 
# 
# http://www.geoscienceontology.org/svu#hasAssociatedProcess

:hasAssociatedProcess a owl:ObjectProperty .
# 
# http://www.geoscienceontology.org/svu#hasContext

:hasContext a owl:ObjectProperty .
# 
# http://www.geoscienceontology.org/svu#hasHeadOperator

:hasHeadOperator a owl:ObjectProperty ;
	rdfs:subPropertyOf :hasOperator .
# 
# http://www.geoscienceontology.org/svu#hasMediumPhenomenon

:hasMediumPhenomenon a owl:ObjectProperty ;
	rdfs:subPropertyOf :hasPhenomenon .
# 
# http://www.geoscienceontology.org/svu#hasObject

:hasObject a owl:ObjectProperty .
# 
# http://www.geoscienceontology.org/svu#hasOperator

:hasOperator a owl:ObjectProperty .
# 
# http://www.geoscienceontology.org/svu#hasPhenomenon

:hasPhenomenon a owl:ObjectProperty .
# 
# http://www.geoscienceontology.org/svu#hasPropertyQuantification

:hasPropertyQuantification a owl:ObjectProperty .
# 
# http://www.geoscienceontology.org/svu#hasPropertyRole

:hasPropertyRole a owl:ObjectProperty .
# 
# http://www.geoscienceontology.org/svu#hasPropertyType

:hasPropertyType a owl:ObjectProperty ;
	rdfs:subPropertyOf :hasType .
# 
# http://www.geoscienceontology.org/svu#hasQuantity

:hasQuantity a owl:ObjectProperty .
# 
# http://www.geoscienceontology.org/svu#hasRootPhenomenon

:hasRootPhenomenon a owl:ObjectProperty ;
	rdfs:subPropertyOf :hasPhenomenon .
# 
# http://www.geoscienceontology.org/svu#hasType

:hasType a owl:ObjectProperty .
# 
# http://www.geoscienceontology.org/svu#isDerivedFrom

:isDerivedFrom a owl:ObjectProperty ;
	rdfs:comment "isDerivedFrom links more specific concepts to more generic concepts. It is a mechanism for linking Individuals in the ontology, bypassing explicitly defined taxonomic class hierarchies." .
# 
# http://www.geoscienceontology.org/svu#quantifiesProcess

:quantifiesProcess a owl:ObjectProperty .
# 
# 
# 
# #################################################################
# #
# #    Data properties
# #
# #################################################################
# 
# 
# http://www.geoscienceontology.org/svu#hasAssignedUnits

:hasAssignedUnits a owl:DatatypeProperty ;
	rdfs:subPropertyOf :hasUnits .
# 
# http://www.geoscienceontology.org/svu#hasMultiplierUnits

:hasMultiplierUnits a owl:DatatypeProperty ;
	rdfs:subPropertyOf :hasUnits .
# 
# http://www.geoscienceontology.org/svu#hasPowerUnits

:hasPowerUnits a owl:DatatypeProperty ;
	rdfs:subPropertyOf :hasUnits .
# 
# http://www.geoscienceontology.org/svu#hasUnits

:hasUnits a owl:DatatypeProperty .
# 
# http://www.geoscienceontology.org/svu#hasValue

:hasValue a owl:DatatypeProperty .
# 
# http://www.geoscienceontology.org/svu#isNoun

:isNoun a owl:DatatypeProperty ;
	rdfs:subPropertyOf owl:topDataProperty .
# 
# 
# 
# #################################################################
# #
# #    Classes
# #
# #################################################################
# 
# 
# http://www.geoscienceontology.org/svu#AbstractionType

:AbstractionType a owl:Class ;
	rdfs:comment "An AbstractionType is an abstraction that is generic and is usually (although not always) specified more precisely in a Variable." .
# 
# http://www.geoscienceontology.org/svu#Attribute

:Attribute a owl:Class ;
	rdfs:comment "An attribute consists of a property-value pair. Attributes are used to narrow the identification of an Actor in a variable." .
# 
# http://www.geoscienceontology.org/svu#Body

:Body a owl:Class ;
	rdfs:subClassOf :BodyType ;
	rdfs:comment "A Body is something that has both a well-defined form and substance." .
# 
# http://www.geoscienceontology.org/svu#BodyPart

:BodyPart a owl:Class ;
	rdfs:subClassOf :Phenomenon ;
	rdfs:comment "A body part is in essence a body. However, it is always a part of a bigger whole and would not come into existence otherwise." .
# 
# http://www.geoscienceontology.org/svu#BodyType

:BodyType a owl:Class ;
	rdfs:subClassOf :Phenomenon ;
	rdfs:comment "A BodyType is the same thing as a Body, except (subjectively) BodyTypes are more generic and usually (although not always) describe a type and are less frequently used as the object of a variable." .
# 
# http://www.geoscienceontology.org/svu#Context

:Context a owl:Class ;
	rdfs:comment "Context provides a phenomenon and a context relationship. It can be attached to any phenomenon to give context." .
# 
# http://www.geoscienceontology.org/svu#ContextPhenomenon

:ContextPhenomenon a owl:Class ;
	rdfs:subClassOf :Phenomenon ;
	rdfs:comment "A Context Phenomenon is used to attach a context to a Root Phenomenon." .
# 
# http://www.geoscienceontology.org/svu#Form

:Form a owl:Class ;
	rdfs:subClassOf :Phenomenon ;
	rdfs:comment "The Form class contains elements which describe the visible shape or configuration of something; it defines the spatial extent of something without defining substance or essence." .
# 
# http://www.geoscienceontology.org/svu#MathematicalAbstraction

:MathematicalAbstraction a owl:Class ;
	rdfs:subClassOf :AbstractionType ;
	rdfs:comment "A mathematical abstraction is any mathematical entity." .
# 
# http://www.geoscienceontology.org/svu#MathematicalAbstractionPart

:MathematicalAbstractionPart a owl:Class ;
	rdfs:subClassOf :MathematicalAbstraction ;
	rdfs:comment "An Abstraction Part is an abstraction that is usually part of another abstraction and is not likely to be found by itself. Examples include apex and center." .
# 
# http://www.geoscienceontology.org/svu#Matter

:Matter a owl:Class ;
	rdfs:subClassOf :MatterType ;
	rdfs:comment "Matter is the substance of which something is made." .
# 
# http://www.geoscienceontology.org/svu#MatterType

:MatterType a owl:Class ;
	rdfs:subClassOf :Phenomenon ;
	rdfs:comment "MatterType can also be thought of as matter. However, unlike Matter, MatterType doesn't provide the essence of the substance of which something is made." .
# 
# http://www.geoscienceontology.org/svu#MediumPhenomenon

:MediumPhenomenon a owl:Class ;
	rdfs:subClassOf :Phenomenon ;
	rdfs:comment "a MediumPhenomenon is a Phenomenon that has two Phenomena for measurement, a root and a medium." .
# 
# http://www.geoscienceontology.org/svu#Operator

:Operator a owl:Class ;
	rdfs:comment "An operator is a mathematical operation that can be performed on a quantity." .
# 
# http://www.geoscienceontology.org/svu#OperatorQuantitativeProperty

:OperatorQuantitativeProperty a owl:Class ;
	rdfs:subClassOf :QuantitativeProperty ;
	rdfs:comment "OperatorQuantitativeProperty is the set of Properies that involve an Operator. This class is not essentially different from a QuantitativeProperty. However, at the moment it is distinguished in the ontology as those QuantitativeProperties that are associated with a hasOperator relationship." .
# 
# http://www.geoscienceontology.org/svu#Part

:Part a owl:Class ;
	rdfs:comment "A part has no essence without being attached to a Body, Form or some other Phenomenon. A Part must be attached to one of these before being included in a variable. Examples include top, bottom, side, core, and subskin." .
# 
# http://www.geoscienceontology.org/svu#Phenomenon

:Phenomenon a owl:Class .
# 
# http://www.geoscienceontology.org/svu#PhysicalAbstraction

:PhysicalAbstraction a owl:Class ;
	rdfs:subClassOf :MathematicalAbstraction ;
	rdfs:comment "A Physical Abstraction is a Mathematical abstraction that is applied to a physical phenomenon. Examples include wheelbase and shoreline." .
# 
# http://www.geoscienceontology.org/svu#Process

:Process a owl:Class ;
	rdfs:comment "A process is something that happens, whether in one step or multiple steps. A process refers specifically to the actions of something. A process along with all of its actors, their roles, etc. is a Phenomenon." .
# 
# http://www.geoscienceontology.org/svu#Property

:Property a owl:Class ;
	rdfs:comment "A property is a quality or characteristic of something. A property differs from an attribute in that it is not attached to a value. As an example, 'color' is a property of eyes, while 'brown color' is an attribute of a particular eye. A property is shorthand for a Qualitative Property. Quantitative properties are Qualitative Properties that have been quantified." .
# 
# http://www.geoscienceontology.org/svu#PropertyQuantification

:PropertyQuantification a owl:Class ;
	rdfs:comment "A property quantification is a method for quantifying a property. Examples include index, code, and scale." .
# 
# http://www.geoscienceontology.org/svu#PropertyRole

:PropertyRole a owl:Class ;
	rdfs:comment "A property role provide information about the role a property plays in a larger context. Examples of property roles include exponent, parameter, and coefficient." .
# 
# http://www.geoscienceontology.org/svu#PropertyType

:PropertyType a owl:Class ;
	rdfs:comment "A property type denotes the type of a quantity and is associated with Quantitative Properties. Examples include scalar, vector, tensor, and field." .
# 
# http://www.geoscienceontology.org/svu#QuantitativeProperty

:QuantitativeProperty a owl:Class ;
	rdfs:subClassOf :Property , _:genid1 .

_:genid1 a owl:Restriction ;
	owl:onProperty :hasPropertyQuantification ;
	owl:allValuesFrom :PropertyQuantification .

:QuantitativeProperty rdfs:subClassOf _:genid2 .

_:genid2 a owl:Restriction ;
	owl:onProperty :hasPropertyRole ;
	owl:allValuesFrom :PropertyRole .

:QuantitativeProperty rdfs:subClassOf _:genid3 .

_:genid3 a owl:Restriction ;
	owl:onProperty :hasPropertyType ;
	owl:allValuesFrom :PropertyType .

:QuantitativeProperty rdfs:subClassOf _:genid4 .

_:genid4 a owl:Restriction ;
	owl:onProperty :isDerivedFrom ;
	owl:allValuesFrom :Property .

:QuantitativeProperty rdfs:comment "A Quantitative Property (Quantity in shorthand) is a property that has been quantified in some way." .
# 
# http://www.geoscienceontology.org/svu#Relationship

:Relationship a owl:Class ;
	rdfs:comment "This is the class of spatial and temporal relationships between phenomena used to build variables." .
# 
# http://www.geoscienceontology.org/svu#Role

:Role a owl:Class ;
	rdfs:comment "The role class contains the roles that different phenomena may take depending on context. It does not identify the substance or form that identifies the physical existence of a thing; rather, it identifies the ways in which the actions of something determine the role it is playing as part of the bigger picture. Examples include trash, crop, byproduct, and projectile." .
# 
# http://www.geoscienceontology.org/svu#Trajectory

:Trajectory a owl:Class ;
	rdfs:comment "Trajectory identifies the path taken by a body undergoing the process of motion in space." .
# 
# http://www.geoscienceontology.org/svu#TrajectoryDirection

:TrajectoryDirection a owl:Class ;
	rdfs:comment "Associated with a trajectory, indicated direction." .
# 
# http://www.geoscienceontology.org/svu#Variable

:Variable a owl:Class .
# 
# Generated by the OWL API (version 4.2.5.20160517-0735) https://github.com/owlcs/owlapi
