@prefix : <http://www.geoscienceontology.org/svu#> .
@prefix owl: <http://www.w3.org/2002/07/owl#> .
@prefix rdf: <http://www.w3.org/1999/02/22-rdf-syntax-ns#> .
@prefix xml: <http://www.w3.org/XML/1998/namespace> .
@prefix xsd: <http://www.w3.org/2001/XMLSchema#> .
@prefix rdfs: <http://www.w3.org/2000/01/rdf-schema#> .
@base <http://www.geoscienceontology.org/svu> .

<http://www.geoscienceontology.org/svu> rdf:type owl:Ontology ;
                                         rdfs:comment "Scientific Variables Ontology: Upper Ontology. This Ontology defines the core classes and design patterns for building variables. Class individuals are declared in the lower ontology." .

#################################################################
#    Annotation properties
#################################################################

###  http://www.geoscienceontology.org/svu#hasAssociatedWikipediaPage
:hasAssociatedWikipediaPage rdf:type owl:AnnotationProperty ;
                            rdfs:comment "Points to a URL identifying a related Wikipedia Page. Wikipedia pages are used to retrieve narrative, documentation information about entitites in the ontology when available. Wikipedia URLs are not equivalent IRIs." ;
                            rdfs:subPropertyOf rdfs:comment .


###  http://www.geoscienceontology.org/svu#hasNominalization
:hasNominalization rdf:type owl:AnnotationProperty ;
                   rdfs:subPropertyOf rdfs:label .


###  http://www.geoscienceontology.org/svu#hasPresentParticiple
:hasPresentParticiple rdf:type owl:AnnotationProperty ;
                      rdfs:subPropertyOf rdfs:label .


#################################################################
#    Object Properties
#################################################################

###  http://www.geoscienceontology.org/svu#hasHeadOperator
:hasHeadOperator rdf:type owl:ObjectProperty ;
                 rdfs:subPropertyOf :hasOperator .


###  http://www.geoscienceontology.org/svu#hasOperator
:hasOperator rdf:type owl:ObjectProperty .


###  http://www.geoscienceontology.org/svu#hasPropertyQuantification
:hasPropertyQuantification rdf:type owl:ObjectProperty .


###  http://www.geoscienceontology.org/svu#hasPropertyRole
:hasPropertyRole rdf:type owl:ObjectProperty .


###  http://www.geoscienceontology.org/svu#hasPropertyType
:hasPropertyType rdf:type owl:ObjectProperty ;
                 rdfs:subPropertyOf :hasType .


###  http://www.geoscienceontology.org/svu#hasType
:hasType rdf:type owl:ObjectProperty .


###  http://www.geoscienceontology.org/svu#isDerivedFrom
:isDerivedFrom rdf:type owl:ObjectProperty ;
               rdfs:comment "isDerivedFrom links more specific concepts to more generic concepts. It is a mechanism for linking Individuals in the ontology, bypassing explicitly defined taxonomic class hierarchies." .


###  http://www.geoscienceontology.org/svu#quantifiesProcess
:quantifiesProcess rdf:type owl:ObjectProperty .


#################################################################
#    Data properties
#################################################################

###  http://www.geoscienceontology.org/svu#hasAssignedUnits
:hasAssignedUnits rdf:type owl:DatatypeProperty ;
                  rdfs:subPropertyOf :hasUnits .


###  http://www.geoscienceontology.org/svu#hasMultiplierUnits
:hasMultiplierUnits rdf:type owl:DatatypeProperty ;
                    rdfs:subPropertyOf :hasUnits .


###  http://www.geoscienceontology.org/svu#hasPowerUnits
:hasPowerUnits rdf:type owl:DatatypeProperty ;
               rdfs:subPropertyOf :hasUnits .


###  http://www.geoscienceontology.org/svu#hasUnits
:hasUnits rdf:type owl:DatatypeProperty .


###  http://www.geoscienceontology.org/svu#hasValue
:hasValue rdf:type owl:DatatypeProperty .


###  http://www.geoscienceontology.org/svu#isNoun
:isNoun rdf:type owl:DatatypeProperty ;
        rdfs:subPropertyOf owl:topDataProperty .


#################################################################
#    Classes
#################################################################

###  http://www.geoscienceontology.org/svu#Attribute
:Attribute rdf:type owl:Class ;
           rdfs:comment "An attribute consists of a property-value pair. Attributes are used to narrow the identification of an Actor in a variable." .


###  http://www.geoscienceontology.org/svu#Body
:Body rdf:type owl:Class ;
      rdfs:subClassOf :BodyType ;
      rdfs:comment "A Body is something that has both a well-defined form and substance." .


###  http://www.geoscienceontology.org/svu#BodyPart
:BodyPart rdf:type owl:Class ;
          rdfs:comment "A body part is in essence a body. However, it is always a part of a bigger whole and would not come into existence otherwise." .


###  http://www.geoscienceontology.org/svu#BodyType
:BodyType rdf:type owl:Class ;
          rdfs:comment "A BodyType is the same thing as a Body, except (subjectively) BodyTypes are more generic and usually (although not always) describe a type and are less frequently used as the object of a variable." .


###  http://www.geoscienceontology.org/svu#Form
:Form rdf:type owl:Class ;
      rdfs:comment "The Form class contains elements which describe the visible shape or configuration of something; it defines the spatial extent of something without defining substance or essence." .


###  http://www.geoscienceontology.org/svu#Matter
:Matter rdf:type owl:Class ;
        rdfs:subClassOf :MatterType ;
        rdfs:comment "Matter is the substance of which something is made." .


###  http://www.geoscienceontology.org/svu#MatterType
:MatterType rdf:type owl:Class ;
            rdfs:comment "MatterType can also be thought of as matter. However, unlike Matter, MatterType doesn't provide the essence of the substance of which something is made." .


###  http://www.geoscienceontology.org/svu#Operator
:Operator rdf:type owl:Class ;
          rdfs:comment "An operator is a mathematical operation that can be performed on a quantity." .


###  http://www.geoscienceontology.org/svu#OperatorQuantitativeProperty
:OperatorQuantitativeProperty rdf:type owl:Class ;
                              rdfs:subClassOf :QuantitativeProperty ;
                              rdfs:comment "OperatorQuantitativeProperty is the set of Properies that involve an Operator. This class is not essentially different from a QuantitativeProperty. However, at the moment it is distinguished in the ontology as those QuantitativeProperties that are associated with a hasOperator relationship." .


###  http://www.geoscienceontology.org/svu#Process
:Process rdf:type owl:Class ;
         rdfs:comment "A process is something that happens, whether in one step or multiple steps. A process refers specifically to the actions of something. A process along with all of its actors, their roles, etc. is a Phenomenon." .


###  http://www.geoscienceontology.org/svu#Property
:Property rdf:type owl:Class ;
          rdfs:comment "A property is a quality or characteristic of something. A property differs from an attribute in that it is not attached to a value. As an example, 'color' is a property of eyes, while 'brown color' is an attribute of a particular eye. A property is shorthand for a Qualitative Property. Quantitative properties are Qualitative Properties that have been quantified." .


###  http://www.geoscienceontology.org/svu#PropertyQuantification
:PropertyQuantification rdf:type owl:Class ;
                        rdfs:comment "A property quantification is a method for quantifying a property. Examples include index, code, and scale." .


###  http://www.geoscienceontology.org/svu#PropertyRole
:PropertyRole rdf:type owl:Class ;
              rdfs:comment "A property role provide information about the role a property plays in a larger context. Examples of property roles include exponent, parameter, and coefficient." .


###  http://www.geoscienceontology.org/svu#PropertyType
:PropertyType rdf:type owl:Class ;
              rdfs:comment "A property type denotes the type of a quantity and is associated with Quantitative Properties. Examples include scalar, vector, tensor, and field." .


###  http://www.geoscienceontology.org/svu#QuantitativeProperty
:QuantitativeProperty rdf:type owl:Class ;
                      rdfs:subClassOf :Property ,
                                      [ rdf:type owl:Restriction ;
                                        owl:onProperty :hasPropertyQuantification ;
                                        owl:allValuesFrom :PropertyQuantification
                                      ] ,
                                      [ rdf:type owl:Restriction ;
                                        owl:onProperty :hasPropertyRole ;
                                        owl:allValuesFrom :PropertyRole
                                      ] ,
                                      [ rdf:type owl:Restriction ;
                                        owl:onProperty :hasPropertyType ;
                                        owl:allValuesFrom :PropertyType
                                      ] ,
                                      [ rdf:type owl:Restriction ;
                                        owl:onProperty :isDerivedFrom ;
                                        owl:allValuesFrom :Property
                                      ] ;
                      rdfs:comment "A Quantitative Property (Quantity in shorthand) is a property that has been quantified in some way." .


###  http://www.geoscienceontology.org/svu#Relationship
:Relationship rdf:type owl:Class ;
              rdfs:comment "This is the class of spatial and temporal relationships between phenomena used to build variables." .


###  http://www.geoscienceontology.org/svu#Role
:Role rdf:type owl:Class ;
      rdfs:comment "The role class contains the roles that different phenomena may take depending on context. It does not identify the substance or form that identifies the physical existence of a thing; rather, it identifies the ways in which the actions of something determine the role it is playing as part of the bigger picture. Examples include trash, crop, byproduct, and projectile." .


###  http://www.geoscienceontology.org/svu#Trajectory
:Trajectory rdf:type owl:Class ;
            rdfs:comment "Trajectory identifies the path taken by a body undergoing the process of motion in space." .


###  http://www.geoscienceontology.org/svu#TrajectoryDirection
:TrajectoryDirection rdf:type owl:Class ;
                     rdfs:comment "Associated with a trajectory, indicated direction." .


###  Generated by the OWL API (version 4.2.8.20170104-2310) https://github.com/owlcs/owlapi
